refactor: add and make use of swaps congr theorem
also makes initial performance improvments

Signed-off-by: Somo S. <chisomo@mombo.solutions>

SwapsPerm.lean
@@ -12,31 +12,20 @@
 import Std.Data.Array.Lemmas
 
 section subst_lemmas
-section comm
-@[simp] private theorem fin_cast_val_comm (h1 : n = n' := by first | trivial | simp_all) (h2 : n' = n'' := by first | trivial | simp_all) (i : Fin n) : ((h1 ▸ h2 : n = n'') ▸ i : Fin n'')  =  (h2 ▸ (h1 ▸ i) : Fin n'') := by cases h1; rfl
-@[simp] private theorem prod_fin_cast_val_comm (h1 : n = n' := by first | trivial | simp_all) (h2 : n' = n'' := by first | trivial | simp_all) (p : Fin n × Fin n) : ((h1 ▸ h2 : n = n'') ▸ p : Fin n'' × Fin n'')  =  (h2 ▸ (h1 ▸ p) : Fin n'' × Fin n'') := by cases h1; rfl
 
-@[simp] private theorem list_prod_fin_cast_val_comm (h1 : n = n' := by first | trivial | simp_all) (h2 : n' = n'' := by first | trivial | simp_all) (ps: List (Fin n × Fin n)) : ((h1.symm ▸ h2 : n = n'') ▸ ps : List (Fin n'' × Fin n''))  =  (h2 ▸ (h1 ▸ ps) : List (Fin n'' × Fin n'')) := by cases h1; rfl
+private theorem list_prod_fin_cast_val_comm (h1 : n = n') (h2 : n' = n'') (ps: List (Fin n × Fin n)) : ((h1.symm ▸ h2 : n = n'') ▸ ps : List (Fin n'' × Fin n''))  =  (h2 ▸ (h1 ▸ ps) : List (Fin n'' × Fin n'')) := by cases h1; rfl
 
-end comm
+private theorem fin_cast_val (h : n = n') (i : Fin n) : h ▸ i = ⟨i.1, h ▸ i.2⟩ := by cases h; rfl
 
-@[simp] private theorem gen_cast_val_inverse {motive : Nat → Sort u} (h : n = n' := by first | trivial | simp_all)  (x : motive n) : h.symm ▸ h ▸ x = x := by cases h; rfl
+private theorem prod_fin_cast_val (h : n = n') (p : Fin n × Fin n) : h ▸ p = (h ▸ p.1, h ▸ p.2) := by cases h; rfl
 
-@[simp] private theorem fin_cast_val (h : n = n' := by first | trivial | simp_all) (i : Fin n) : h ▸ i = ⟨i.1, h ▸ i.2⟩ := by cases h; rfl
-
-
-@[simp] private theorem prod_fin_cast_val (h : n = n' := by first | trivial | simp_all) (p : Fin n × Fin n) : h ▸ p = (h ▸ p.1, h ▸ p.2) := by cases h; rfl
-
-
-@[simp] private theorem list_prod_fin_cast_val (h : n = n' := by first | trivial | simp_all) (ps : List (Fin n × Fin n)) : h ▸ ps = ps.map (fun p => ⟨⟨p.1.1, h ▸ p.1.2⟩, ⟨p.2.1, h ▸ p.2.2⟩⟩) :=
+private theorem list_prod_fin_cast_val (h : n = n') (ps : List (Fin n × Fin n)) : h ▸ ps = ps.map (fun p => ⟨⟨p.1.1, h ▸ p.1.2⟩, ⟨p.2.1, h ▸ p.2.2⟩⟩) :=
   have aux : h ▸ ps = ps.map (h ▸ ·) := by cases h; simp -- ; apply Eq.symm; induction ps <;> simp_all
-  by simp_all
+  by simp_all only [prod_fin_cast_val, fin_cast_val]
 
-@[simp] private theorem list_prod_fin_cast_val_append (h : n = n' := by first | trivial | simp_all) (ps ps': List (Fin n × Fin n)) : h ▸ (ps ++ ps') =  (h ▸ ps) ++ (h ▸ ps') := by simp_all
+private theorem list_prod_fin_cast_val_append (h : n = n') (ps ps': List (Fin n × Fin n)) : h ▸ (ps ++ ps') =  (h ▸ ps) ++ (h ▸ ps') := by simp_all only [list_prod_fin_cast_val, List.map_append]
 
-
-@[simp] private theorem list_prod_fin_cast_val_reverse {ps : List (Fin n × Fin n)} (h : n = n' := by first | trivial | simp_all) : h ▸ (ps.reverse) = (h ▸ ps).reverse := by cases h; rfl
-
+private theorem list_prod_fin_cast_val_reverse {ps : List (Fin n × Fin n)} (h : n = n') : h ▸ (ps.reverse) = (h ▸ ps).reverse := by cases h; rfl
 
 end subst_lemmas
 
@@ -45,7 +34,7 @@ namespace Array
 
 variable {a a': Array α} {i j p: Fin a.size}
 
-@[simp] def swaps (a : Array α) : List (Fin a.size × Fin a.size) → Array α
+def swaps (a : Array α) : List (Fin a.size × Fin a.size) → Array α
   | [] => a
   | (i, j) :: ijs =>
     have : (a.swap i j).size = a.size := a.size_swap _ _
@@ -54,14 +43,15 @@ variable {a a': Array α} {i j p: Fin a.size}
     swaps (a.swap i j) (ijs.map (fun p => ⟨⟨p.1.1, this.symm ▸ p.1.2⟩, ⟨p.2.1, this.symm ▸ p.2.2⟩⟩))
 termination_by l => l.length
 
-
-
-@[simp] theorem swaps_zero_eq_swap : a.swaps [] = a := by simp
-@[simp] theorem swaps_one_eq_swap : a.swaps [(i, j)] = a.swap i j := by simp
-@[simp] theorem swaps_two_eq_swap_swap {i1 j1 i2 j2 : Fin a.size}: a.swaps [(i1, j1),(i2, j2)] = (a.swap i1 j1).swap (⟨i2.1, (a.size_swap _ _).symm ▸ i2.2⟩) ⟨j2.1, (a.size_swap _ _).symm ▸ j2.2⟩ :=  by simp
+@[simp] theorem swaps_zero_eq_swap : a.swaps [] = a := by simp [swaps]
+@[simp] theorem swaps_one_eq_swap : a.swaps [(i, j)] = a.swap i j := by simp [swaps]
+@[simp] theorem swaps_two_eq_swap_swap {i1 j1 i2 j2 : Fin a.size}: a.swaps [(i1, j1),(i2, j2)] = (a.swap i1 j1).swap (⟨i2.1, (a.size_swap _ _).symm ▸ i2.2⟩) ⟨j2.1, (a.size_swap _ _).symm ▸ j2.2⟩ :=  by simp [swaps]
 
 @[simp] theorem swaps_two_id : a.swaps [c,c]  = a := by let (i, j) := c; simp
 
+theorem swaps_congr {n : Nat} (a1 a2 : Array α) (l : List (Fin n × Fin n)) (ha1 : n = a1.size) (ha2 : n = a2.size) (heq : a1 = a2) : a1.swaps (ha1 ▸ l) = a2.swaps (ha2 ▸ l) := by
+  have : {val := a1, property := ha1 : Subtype (n = ·.size)} = {val := a2, property := ha2: Subtype (n = ·.size)} := Subtype.eq heq
+  apply congrArg (fun x => swaps x.1 (x.2 ▸ l)) this
 
 @[simp] theorem size_swaps (a : Array α) : ∀ {l}, (a.swaps l).size = a.size
   | [] => by simp
@@ -69,57 +59,63 @@ termination_by l => l.length
 termination_by l => l.length
 
 
-@[simp] theorem swaps_append (a : Array α) (l l': List (Fin a.size × Fin a.size)) : (a.swaps l).swaps (a.size_swaps.symm ▸ l') = a.swaps (l ++ l') :=
+-- set_option trace.profiler true in
+attribute [simp] list_prod_fin_cast_val in -- required for termination proof
+theorem swaps_append (a : Array α) (l l': List (Fin a.size × Fin a.size)) : (a.swaps l).swaps (a.size_swaps.symm ▸ l') = a.swaps (l ++ l') :=
   match l with
-  | [] =>
-    suffices swaps (swaps a []) l' = swaps a l' by simp_all
+  | [] => by
     have : a.swaps [] = a :=  a.swaps_zero_eq_swap
-    congrArg (fun _ => swaps a l') this
-
+    have : (a.swaps []).swaps l' = a.swaps l' := congrArg (fun _ => swaps a l') this
+    simp_all only [List.nil_append]
   | (i, j) :: ijs =>
     have hs : (a.swap i j).size = a.size := a.size_swap _ _
     have hs's: ((a.swap i j).swaps (hs.symm ▸ ijs)).size = (a.swap i j).size := (a.swap i j).size_swaps
-    have hss : ((a.swap i j).swaps (hs.symm ▸ ijs)).size = a.size := hs's.symm ▸ hs
+    have hss : ((a.swap i j).swaps (hs.symm ▸ ijs)).size = a.size := Trans.trans hs's hs
 
-    have ih : ((a.swap i j).swaps (hs.symm ▸ ijs)).swaps (hs's.symm ▸ (hs.symm ▸ l')) = (a.swap i j).swaps ((hs.symm ▸ ijs) ++ (hs.symm ▸ l')) := swaps_append (a.swap i j) (hs.symm ▸ ijs) (hs.symm ▸ l')
+    have ih : ((a.swap i j).swaps (hs.symm ▸ ijs)).swaps (hs's.symm ▸ (hs.symm ▸ l')) = (a.swap i j).swaps ((hs.symm ▸ ijs) ++ (hs.symm ▸ l')) := by apply swaps_append (a.swap i j) (hs.symm ▸ ijs) (hs.symm ▸ l') -- TODO: using apply tactic to speed it up. But shouldnt otherwise be necessary
 
     have h_suff : ((a.swap i j).swaps (hs.symm ▸ ijs)).swaps (hss.symm ▸ l') = (a.swap i j).swaps (hs.symm ▸ (ijs ++ l')) :=
-      (list_prod_fin_cast_val_comm (hs.symm) (hs's.symm) (l')).symm ▸ ((list_prod_fin_cast_val_append hs.symm (ijs) (l')).symm ▸ ih)
+      (list_prod_fin_cast_val_comm (hs.symm) (hs's.symm) (l')).symm
+      ▸ (list_prod_fin_cast_val_append hs.symm (ijs) (l')).symm
+      ▸ ih
 
-    have : (a.swaps ((i, j) :: ijs)) = ((a.swap i j).swaps (hs.symm ▸ ijs)) := by simp
-    have : {val := (a.swaps ((i, j) :: ijs)), property := a.size_swaps.symm : Subtype (a.size = ·.size)} = {val := ((a.swap i j).swaps (hs.symm ▸ ijs)), property := hss.symm : Subtype (a.size = ·.size)} := Subtype.eq this
+    have : (a.swaps ((i, j) :: ijs)).swaps (a.size_swaps.symm ▸ l') = ((a.swap i j).swaps (hs.symm ▸ ijs)).swaps (hss.symm ▸ l') := by apply swaps_congr ; simp only [swaps, list_prod_fin_cast_val]
 
-    have heq : (a.swaps ((i, j) :: ijs)).swaps (a.size_swaps.symm ▸ l') = ((a.swap i j).swaps (hs.symm ▸ ijs)).swaps (hss.symm ▸ l') := congrArg (fun x => swaps x.1 (x.2 ▸ l')) this
-
-      show (a.swaps ((i, j) :: ijs)).swaps (a.size_swaps.symm ▸ l') = a.swaps ((i, j) :: ijs ++ l') by simp_all
+    by simp_all only [list_prod_fin_cast_val, swaps, List.cons_append]
   termination_by l.length
 
 set_option maxHeartbeats 5000000 in
-@[simp] theorem swaps_cancel (a : Array α) (l : List (Fin a.size × Fin a.size)) : a.swaps (l ++ l.reverse) = a :=
+attribute [simp] list_prod_fin_cast_val in -- required for termination proof
+theorem swaps_cancel (a : Array α) (l : List (Fin a.size × Fin a.size)) : a.swaps (l ++ l.reverse) = a :=
   match l with
-  | [] => by simp
+  | [] => by simp only [List.reverse_nil, List.append_nil, swaps]
 
   | c :: cs =>
 
-    have hs' : (a.swaps [c]).size = a.size := a.size_swaps
+    have hs' : (a.swaps [c]).size = a.size := by rw [size_swaps] -- a.size_swaps
 
-    have hs'' : ((a.swaps [c]).swaps (hs'.symm ▸ (cs ++ cs.reverse))).size = (a.swaps [c]).size := (a.swaps [c]).size_swaps
-    have hs : ((a.swaps [c]).swaps (hs'.symm ▸ (cs ++ cs.reverse))).size = a.size :=  hs''.symm ▸ hs'
+    have hs'' : ((a.swaps [c]).swaps (hs'.symm ▸ (cs ++ cs.reverse))).size = (a.swaps [c]).size := by rw [size_swaps] -- (a.swaps [c]).size_swaps
+    have hs : ((a.swaps [c]).swaps (hs'.symm ▸ (cs ++ cs.reverse))).size = a.size :=  by simp only [size_swaps] -- hs''.symm ▸ hs'
 
     have : ((a.swaps [c]).swaps ((hs'.symm ▸ cs) ++ (hs'.symm ▸ cs).reverse)) = (a.swaps [c]) := swaps_cancel (a.swaps [c]) (hs'.symm ▸ cs)
-    have : ((a.swaps [c]).swaps ((hs'.symm ▸ cs) ++ (hs'.symm ▸ cs.reverse))) = (a.swaps [c]) := (list_prod_fin_cast_val_reverse hs'.symm) ▸ this
-    have ih : ((a.swaps [c]).swaps (hs'.symm ▸ (cs ++ cs.reverse))) = (a.swaps [c]) := (list_prod_fin_cast_val_append hs'.symm .. ▸ this)
+    -- have : ((a.swaps [c]).swaps ((hs'.symm ▸ cs) ++ (hs'.symm ▸ cs).reverse)) = (a.swaps [c]) := by exact (swaps_cancel (a.swaps [c]) (hs'.symm ▸ cs))
+    -- have : ((a.swaps [c]).swaps ((hs'.symm ▸ cs) ++ (hs'.symm ▸ cs).reverse)) = (a.swaps [c]) := by /- show_term -/ apply swaps_cancel
+    -- have : ((a.swaps [c]).swaps ((hs'.symm ▸ cs) ++ (hs'.symm ▸ cs).reverse)) = (a.swaps [c]) := by  /- with_reducible -/ exact (swaps_cancel (a.swaps [c]) (hs'.symm ▸ cs))
 
-    have heq_comm : (hs.symm ▸ [c] : List (Fin ((a.swaps [c]).swaps (hs'.symm ▸ (cs ++ cs.reverse))).size × Fin ((a.swaps [c]).swaps (hs'.symm ▸ (cs ++ cs.reverse))).size))  =  (hs''.symm ▸ (hs'.symm ▸ [c]) : List (Fin ((a.swaps [c]).swaps (hs'.symm ▸ (cs ++ cs.reverse))).size × Fin ((a.swaps [c]).swaps (hs'.symm ▸ (cs ++ cs.reverse))).size)) :=  (list_prod_fin_cast_val_comm hs'.symm hs''.symm) [c]
+    have : ((a.swaps [c]).swaps ((hs'.symm ▸ cs) ++ (hs'.symm ▸ cs.reverse))) = (a.swaps [c]) := by rw [(list_prod_fin_cast_val_reverse hs'.symm)]; exact this -- (list_prod_fin_cast_val_reverse hs'.symm) ▸ this
+    have ih : ((a.swaps [c]).swaps (hs'.symm ▸ (cs ++ cs.reverse))) = (a.swaps [c]) := by rw [(list_prod_fin_cast_val_append hs'.symm ..)]; exact this -- (list_prod_fin_cast_val_append hs'.symm .. ▸ this)
 
     calc  a.swaps ((c :: cs) ++ (c :: cs).reverse)
-      _ = a.swaps (      [c] ++ (cs ++ cs.reverse ++ [c])     ) := by simp
-      _ = (a.swaps [c]).swaps ( hs'.symm ▸ (cs ++ cs.reverse ++ [c]) ) := (swaps_append a [c] (cs ++ cs.reverse ++ [c])).symm
-      _ = (a.swaps [c]).swaps ( (hs'.symm ▸ (cs ++ cs.reverse)) ++ (hs'.symm ▸ [c]) ) := by simp
-      _ = ((a.swaps [c]).swaps (hs'.symm ▸ (cs ++ cs.reverse))).swaps  (hs''.symm ▸ (hs'.symm ▸ [c])) := (swaps_append (a.swaps [c])  (hs'.symm ▸ (cs ++ cs.reverse)) (hs'.symm ▸ [c])).symm
-      _ = ((a.swaps [c]).swaps (hs'.symm ▸ (cs ++ cs.reverse))).swaps  (hs.symm ▸ [c]) := by rw [←heq_comm]
-      _ = (a.swaps [c]).swaps  (hs'.symm ▸ [c]) := by congr ; simp
-      _ = a.swaps ([c] ++ [c]) := swaps_append a [c] [c]
+      _ = a.swaps (      [c] ++ (cs ++ cs.reverse ++ [c])     ) := by simp only [List.reverse_cons, List.cons_append, List.append_assoc, List.nil_append]
+      _ = (a.swaps [c]).swaps ( hs'.symm ▸ (cs ++ cs.reverse ++ [c]) ) := by apply Eq.symm ; apply swaps_append -- (swaps_append a [c] (cs ++ cs.reverse ++ [c])).symm
+      _ = (a.swaps [c]).swaps ( (hs'.symm ▸ (cs ++ cs.reverse)) ++ (hs'.symm ▸ [c]) ) := by simp only [list_prod_fin_cast_val, List.map_append]
+      _ = ((a.swaps [c]).swaps (hs'.symm ▸ (cs ++ cs.reverse))).swaps  (hs''.symm ▸ hs'.symm ▸ [c]) := by apply Eq.symm ; apply swaps_append -- (swaps_append (a.swaps [c])  (hs'.symm ▸ (cs ++ cs.reverse)) (hs'.symm ▸ [c])).symm
+
+      -- _ = ((a.swaps [c]).swaps (hs'.symm ▸ (cs ++ cs.reverse))).swaps  (hs.symm ▸ [c]) := by simp only [list_prod_fin_cast_val, List.map] -- FIXME: is slow appox. 6seconds
+      _ = ((a.swaps [c]).swaps (hs'.symm ▸ (cs ++ cs.reverse))).swaps  (hs.symm ▸ [c]) := /- show_term by rw [(list_prod_fin_cast_val_comm hs'.symm hs''.symm [c])] --> FIXME: is slow appox. 9seconds -/ Eq.mpr (id (congrArg (fun _a => swaps (swaps (swaps a [c]) (Eq.symm hs' ▸ (cs ++ List.reverse cs))) (Eq.symm hs'' ▸ Eq.symm hs' ▸ [c]) = swaps (swaps (swaps a [c]) (Eq.symm hs' ▸ (cs ++ List.reverse cs))) _a) (list_prod_fin_cast_val_comm (Eq.symm hs') (Eq.symm hs'') [c]))) (Eq.refl (swaps (swaps (swaps a [c]) (Eq.symm hs' ▸ (cs ++ List.reverse cs))) (Eq.symm hs'' ▸ Eq.symm hs' ▸ [c])))-- FIXME: is appox. 3.5seconds
+
+      _ = (a.swaps [c]).swaps  (hs'.symm ▸ [c]) := swaps_congr ((a.swaps [c]).swaps (hs'.symm ▸ (cs ++ cs.reverse))) (a.swaps [c]) [c] (hs.symm) (hs'.symm) ih
+      _ = a.swaps ([c] ++ [c]) := by apply swaps_append -- swaps_append a [c] [c]
       _ = a := swaps_two_id
 
   termination_by l.length
@@ -147,34 +143,17 @@ theorem of_eq (h : a1 = a2) : a1 ~ a2 := h ▸ refl a1
 
 
 theorem symm (h : a1 ~ a2) : a2 ~ a1 :=
-  have hs : a1.size = a2.size := h.size_eq
-
   let ⟨l, h⟩ := h; -- have h : a2 = (a1.swaps l) := h
 
-  have : ⟨a2, hs⟩ = {val := (a1.swaps l), property := h ▸ hs : Subtype (a1.size = ·.size)} := Subtype.eq h
-
-  have : a2.swaps ((h.symm ▸ a1.size_swaps) ▸ l.reverse) = a1 :=
-    calc a2.swaps ((h.symm ▸ a1.size_swaps) ▸ l.reverse)
-      _ = (a1.swaps l).swaps (a1.size_swaps ▸ l.reverse) := congrArg (fun x => swaps x.1 (x.2 ▸ l.reverse)) this
+  have : a2.swaps ((h.symm ▸ a1.size_swaps) ▸ l.reverse) = a1 := calc
+      _ = (a1.swaps l).swaps (a1.size_swaps ▸ l.reverse) := by apply swaps_congr ; assumption
       _ = a1.swaps (l ++ l.reverse) := swaps_append a1 l l.reverse
       _ = a1 := swaps_cancel a1 l
+
   ⟨(h.symm ▸ a1.size_swaps) ▸ l.reverse, this.symm⟩
 
 
 theorem trans (h1 : a1 ~ a2) (h2 : a2 ~ a3) : a1 ~ a3 :=
-  let swaps_append_gen  (a : Array α) {n n' : Nat} {l : List (Fin n × Fin n)} {l' : List (Fin n' × Fin n')} (hn : n = a.size) (h : n' = n) (hn' : n' = (a.swaps (hn ▸ l)).size) : (a.swaps (hn ▸ l)).swaps (hn' ▸ l') = a.swaps ((hn ▸ l) ++ ((h.symm ▸ hn) ▸ l')) :=
-    let swaps_append_short (a : Array α) (l : List (Fin a.size × Fin a.size)) (l': List (Fin (a.swaps l).size × Fin (a.swaps l).size)) : (a.swaps l).swaps l' = a.swaps (l ++ (a.size_swaps ▸ l')) :=
-      have _ : a.size_swaps.symm ▸ a.size_swaps ▸ l' = l' := gen_cast_val_inverse (motive := (fun n => List (Fin n × Fin n))) ..
-      have _ : (a.swaps l).swaps (a.size_swaps.symm ▸ a.size_swaps ▸ l') = a.swaps (l ++ (a.size_swaps ▸ l')) := swaps_append a l (a.size_swaps ▸ l')
-      by simp_all
-
-    have hss : (a.swaps (hn ▸ l)).size = a.size := Trans.trans (Trans.trans hn'.symm h) hn
-    have : (a.swaps (hn ▸ l)).swaps (hn' ▸ l') = a.swaps ((hn ▸ l) ++ (hss ▸ hn' ▸ l')) := swaps_append_short a (hn ▸ l) (hn' ▸ l')
-
-    have _ : (h.symm ▸ hn) ▸ l' = hss ▸ (hn' ▸ l') := (list_prod_fin_cast_val_comm) l'
-    by simp_all
-
-  ------------------
 
   let ⟨l1, h1'⟩ := h1; -- have h1' : a2 = a1.swaps l1 := h1'
   let ⟨l2, h2'⟩ := h2; -- have h2' : a3 = a2.swaps l2 := h2'
@@ -184,7 +163,10 @@ theorem trans (h1 : a1 ~ a2) (h2 : a2 ~ a3) : a1 ~ a3 :=
   have hs3 : a2.size = (a1.swaps l1).size := Trans.trans hs2 hs1
 
   have h3' : a3 = (a1.swaps l1).swaps ((Trans.trans hs2 hs1) ▸ l2) := h1' ▸ h2'
-  have : (a1.swaps l1).swaps (hs3 ▸ l2) = a1.swaps (l1 ++ (hs2 ▸ l2)) := swaps_append_gen a1 rfl hs2 .. /- hs3 -/
+
+  have : (a1.swaps l1).swaps (hs3 ▸ l2) = a1.swaps (l1 ++ (hs2 ▸ l2)) := calc _
+    _ = (a1.swaps l1).swaps (a1.size_swaps.symm ▸ hs2 ▸ l2) := by simp only [←list_prod_fin_cast_val_comm]
+    _ = a1.swaps (l1 ++ (hs2 ▸ l2)) := a1.swaps_append l1 (hs2 ▸ l2)
 
   have : a3 = a1.swaps (l1 ++ (hs2 ▸ l2)) := Trans.trans h3'  this
 
